Make everything modular

theories/State.v
@@ -7,33 +7,49 @@ From Stdlib Require Import FunctionalExtensionality.
 
 From Forq Require Import Syntax.
 
-Module State (syntax : WordSyntax).
-  Export syntax.
+Module Type StateType (syntax : WordSyntax).
+  Record state : Type := {
+    stack : list N;
+    mem : addr -> N;
+    dict : addr -> syntax.program
+  }.
+End StateType.
 
-  Record state := {
-    stack : list N;         (* data stack *)
-    mem : addr -> N;        (* memory function *)
-    dict : addr -> program (* word dictionary *)
+Module State (syntax : WordSyntax) <: StateType syntax.
+  Record state : Type := {
+    stack : list N;                 (* data stack *)
+    mem : addr -> N;                (* memory function *)
+    dict : addr -> syntax.program   (* word dictionary *)
   }.
 
   Definition empty_mem : (addr -> N) :=
     fun _ => 0.
 
-  Definition empty_dict : (addr -> program) :=
+  Definition empty_dict : (addr -> syntax.program) :=
     fun _ => [].
 End State.
 
 Definition update (mem : addr -> N) (key : addr) (val : N) : (addr -> N) :=
   fun key' => if key' =? key then val else mem key'.
+Notation "m [ k := v ]" := (update m k v).
 
 Definition update_eq : forall mem key val,
-  update mem key val key = val.
+  mem [key := val] key = val.
 Proof.
   intros. unfold update. now rewrite N.eqb_refl.
 Qed.
 
+Definition update_neq : forall mem key1 key2 val,
+  key1 <> key2 ->
+  mem [key1 := val] key2 = mem key2.
+Proof.
+  intros. unfold update.
+  apply not_eq_sym in H.
+  apply N.eqb_neq in H. now rewrite H.
+Qed.
+
 Definition update_shadow : forall mem key val val',
-  update (update mem key val) key val' = update mem key val'.
+  mem [key := val] [key := val'] = mem [key := val'].
 Proof.
   intros. unfold update. apply functional_extensionality. intros.
   now destruct (N.eqb x key).
