theories/Words/Core.v
@@ -1,43 +1,61 @@
 From Stdlib Require Import List.
 Import ListNotations.
+From Stdlib Require Import String.
 From Stdlib Require Import NArith.
 Open Scope N_scope.
 
-From Forq Require Import Result.
-From Forq Require Import Syntax.
-From Forq Require Import State.
+From Forq Require Import Result Syntax State MachineModel.
 From Forq.Words Require Import Word.
 
 Module CoreSyntax <: WordSyntax.
-  Inductive CoreWord : Set := Fetch | Store | Exec.
+  Inductive CoreWord : Set :=
+    | Literal (n : N)       (* put constant integer onto stack - https://forth-standard.org/standard/core/LITERAL *)
+    | Fetch                 (* load from memory address - https://forth-standard.org/standard/core/Fetch *)
+    | Store                 (* store to memory address - https://forth-standard.org/standard/core/Store *)
+    | Exec                  (* execute program - https://forth-standard.org/standard/core/EXECUTE *)
+    .
   Definition word : Type := CoreWord.
+  Coercion Literal : N >-> CoreWord.
 
   Definition program := list word.
 End CoreSyntax.
+Export CoreSyntax.
 
-Module CoreSemantics <: (WordSemantics CoreSyntax).
-  Module St := State CoreSyntax.
-  Export St CoreSyntax.
-
-  Inductive step : state -> CoreWord -> result (state * program) -> Prop :=
+Module CoreSemantics (ST : StateType CoreSyntax) <: (WordSemantics CoreSyntax ST).
+  Import ST.
+  Inductive cstep : state -> CoreWord -> result (state * program) -> Prop :=
+    (* literal *)
+    | StepLiteralOk : forall (s : state) (n : N),
+        cstep s n
+          (Ok ({|stack := n :: s.(stack); mem := s.(mem); dict := s.(dict)|}, []))
     (* fetch *)
     | StepFetchOk : forall (s : state) (addr : addr) (st : list N),
         s.(stack) = addr :: st ->
-        step s Fetch
+        cstep s Fetch
           (Ok ({|stack := s.(mem) addr :: st; 
                 mem := s.(mem); dict := s.(dict)|}, []))
     | StepFetchUnderflow : forall (s : state),
-        s.(stack) = [] -> step s Fetch (Error "fetch: stack underflow")
+        s.(stack) = [] -> cstep s Fetch (Error "fetch: stack underflow")
     (* store *)
     | StepStoreOk : forall (s : state) (val : N) (addr : addr) (st : list N),
         s.(stack) = val :: addr :: st ->
-        step s Store
-          (Ok ({|stack := st; mem := update s.(mem) addr val; 
+        cstep s Store
+          (Ok ({|stack := st; mem := s.(mem)[addr := val]; 
                 dict := s.(dict)|}, []))
     | StepStoreUnderflow : forall (s : state),
         s.(stack) = [] \/ (exists x, s.(stack) = [x]) -> 
-        step s Store (Error "store: stack underflow")
+        cstep s Store (Error "store: stack underflow")
+    (* exec *)
+    | StepExecOk : forall (s : state) (st : list N) (prog_addr : addr),
+        s.(stack) = prog_addr :: st ->
+        cstep s Exec (Ok ({|stack := st; mem := s.(mem); dict := s.(dict)|}, 
+                          s.(dict) prog_addr))
+    | StepExecUnderflow : forall (s : state),
+        s.(stack) = [] ->
+        cstep s Exec (Error "exec: stack underflow")
   .
 
-  Definition cstep := step.
+  Definition step := cstep.
 End CoreSemantics.
+
+
