theories/examples/loadstore.v
@@ -1,35 +1,63 @@
-From Stdlib Require Import NArith.
-Open Scope N_scope.
-From Stdlib Require Import List.
-Import ListNotations.
-
 From Forq Require Import Auto.
 From Forq.Words Require Import Core.
 
-Module Auto := Automation CoreSyntax CoreSemantics.
+Module ST := State CoreSyntax.
+Module SMX := CoreSemantics ST.
+
+Module Auto := Automation CoreSyntax ST SMX MM8.
 Import Auto.
 
-Definition loadstore : program := [Fetch; Store].
+Definition loadstore (addr : word) (val : word) : program := 
+  [addr; val; Store; addr; addr; Fetch; Store].
 
-Theorem loadstore_ident : forall addr val dict, 
+Theorem loadstore_correct : forall (addr val : N) mem dict,
+  mem_well_typed mem ->
+  val < 2^w ->
   pmstep 
-    {| stack := [addr; addr]; mem := update empty_mem addr val; dict := dict |}
-    loadstore
-    {| stack := []; mem := update empty_mem addr val; dict := dict |}.
+    {| stack := []; mem := mem; dict := dict |}
+    (loadstore addr val)
+    {| stack := []; mem := mem[addr := val]; dict := dict |}.
 Proof.
   intros. unfold loadstore.
   eapply PMStepMulti.
-  - constructor. reflexivity.
-  - simpl. rewrite update_eq. eapply PMStepMulti.
-    -- constructor. reflexivity.
-    -- simpl. rewrite update_shadow. apply PMStepRefl.
+    constructor.
+    now cbv [mem].
+  simpl. eapply PMStepMulti.
+    constructor.
+    now cbv [mem].
+  simpl. eapply PMStepMulti.
+    constructor. reflexivity.
+    cbv [mem]. now apply mem_well_typed_update.
+  simpl. eapply PMStepMulti.
+    constructor.
+    cbv [mem]. now apply mem_well_typed_update.
+  simpl. eapply PMStepMulti.
+    constructor.
+    cbv [mem]. now apply mem_well_typed_update.
+  simpl. eapply PMStepMulti.
+    constructor. reflexivity.
+    cbv [mem]. now apply mem_well_typed_update.
+  simpl. eapply PMStepMulti.
+    constructor. reflexivity.
+    cbv [mem]. apply mem_well_typed_update.
+      now apply mem_well_typed_update.
+      now rewrite update_eq.
+  simpl. rewrite update_eq. rewrite update_shadow. apply PMStepRefl.
 Qed.
 
-Theorem loadstore_ident' : forall addr val dict, 
+Theorem loadstore_correct' : forall (addr val : N) mem dict,
+  mem_well_typed mem ->
+  val < 2^w ->
   pmstep 
-    {| stack := [addr; addr]; mem := update empty_mem addr val; dict := dict |}
-    loadstore
-    {| stack := []; mem := update empty_mem addr val; dict := dict |}.
+    {| stack := []; mem := mem; dict := dict |}
+    (loadstore addr val)
+    {| stack := []; mem := mem[addr := val]; dict := dict |}.
 Proof.
-  intros. unfold loadstore. step (). step ().
+  intros. unfold loadstore.
+  (* store *)
+  step (). step (). step ().
+  (* fetch *) 
+  step (). step (). step ().
+  (* store *)
+  step ().
 Qed.
