theories/MachineModel.v
@@ -1,0 +1,34 @@
+From Stdlib Require Import NArith.
+
+From Forq Require Import Syntax State.
+
+Module Type MachineModel (syntax : WordSyntax).
+  Parameter w : N.
+
+  Definition mem_well_typed (mem : addr -> N) : Prop :=
+    forall (a : addr), mem a < 2^w.
+End MachineModel.
+
+Module MM8 (syntax : WordSyntax) <: MachineModel syntax.
+  Definition w := 8.
+  Definition mem_well_typed (mem : addr -> N) : Prop :=
+    forall (a : addr), mem a < 2^w.
+End MM8.
+
+Module MM16 (syntax : WordSyntax) <: MachineModel syntax.
+  Definition w := 16.
+  Definition mem_well_typed (mem : addr -> N) : Prop :=
+    forall (a : addr), mem a < 2^w.
+End MM16.
+
+Module MM32 (syntax : WordSyntax) <: MachineModel syntax.
+  Definition w := 32.
+  Definition mem_well_typed (mem : addr -> N) : Prop :=
+    forall (a : addr), mem a < 2^w.
+End MM32.
+
+Module MM64 (syntax : WordSyntax) <: MachineModel syntax.
+  Definition w := 64.
+  Definition mem_well_typed (mem : addr -> N) : Prop :=
+    forall (a : addr), mem a < 2^w.
+End MM64.
