theories/ProgramSemantics.v
@@ -1,18 +1,23 @@
 From Stdlib Require Import List.
 Import ListNotations.
 
-From Forq Require Import Syntax.
-From Forq Require Import Result.
+From Forq Require Import Result State Syntax MachineModel.
 From Forq.Words Require Import Word.
 
-Module SmallStep (syntax : WordSyntax) (semantics : WordSemantics syntax).
-  Export syntax semantics.
+Module SmallStep (syntax : WordSyntax)
+                 (ST : StateType syntax)
+                 (semantics : WordSemantics syntax ST) 
+                 (model : MachineModel).
+  Module MM := model syntax.
+  Export syntax ST semantics MM.
 
+  Definition nilprog : program := [].
   Inductive pmstep : state -> program -> state -> Prop :=
-  | PMStepRefl : forall s prog,
-      pmstep s prog s
+  | PMStepRefl : forall s,
+      pmstep s nilprog s
   | PMStepMulti : forall wrd p p' s1 s2 s3,
-      cstep s1 wrd (Ok (s2, p')) ->
+      step s1 wrd (Ok (s2, p')) ->
+      mem_well_typed s2.(mem) ->
       pmstep s2 (p' ++ p) s3 ->
       pmstep s1 (wrd :: p) s3.
 End SmallStep.
