theories/Theory.v
@@ -1,0 +1,19 @@
+From Stdlib Require Import NArith.
+From Forq Require Import Syntax MachineModel State.
+
+Module ForqTheory (syntax : WordSyntax) (MM : MachineModel syntax).
+Import MM.
+
+Lemma mem_well_typed_update : forall mem addr val,
+  mem_well_typed mem ->
+  val < 2^w ->
+  mem_well_typed (mem[addr := val]).
+Proof.
+  intros. unfold mem_well_typed in *.
+  intros. destruct (N.eq_dec a addr).
+  - subst. rewrite update_eq. assumption.
+  - rewrite update_neq by (symmetry; assumption).
+    apply H.
+Qed.
+
+End ForqTheory.
