theories/Words/Word.v
@@ -1,10 +1,5 @@
-From Forq Require Import Syntax.
-From Forq Require Import State.
-From Forq Require Import Result.
+From Forq Require Import Result Syntax State MachineModel.
 
-Module Type WordSemantics (syntax : WordSyntax).
-  Module St := State syntax.
-  Export St syntax.
-
-  Parameter cstep : state -> word -> result (state * program) -> Prop.
+Module Type WordSemantics (syntax : WordSyntax) (ST : StateType syntax).
+  Parameter step : ST.state -> syntax.word -> result (ST.state * syntax.program) -> Prop.
 End WordSemantics.
